discrete/AsymptoticBB.lean
@@ -1,4 +1,5 @@
 import AsymptoticBB.Main
 import AsymptoticBB.SemanticCore
 import AsymptoticBB.Basic.CSPHom
+import AsymptoticBB.Basic.Intendable
 import AsymptoticBB.Tests.Sanity
